Lemma 3 from paper

Ranking.thy
@@ -5,8 +5,13 @@ theory Ranking
     "List-Index.List_Index"
 begin
 
+sledgehammer_params [provers = e z3 spass cvc4 vampire]
+
 lemma vs_empty[simp]: "Vs {} = {}"
   by (simp add: Vs_def)
+
+lemma vs_union[simp]: "Vs (A \<union> B) = Vs A \<union> Vs B"
+  unfolding Vs_def by simp
 
 lemma graph_abs_empty[simp]: "graph_abs {}"
   by (simp add: graph_abs_def)
@@ -23,14 +28,40 @@ lemma graph_abs_compr[intro]: "u \<notin> ns \<Longrightarrow> finite ns \<Longr
 lemma matching_empty[simp]: "matching {}"
   unfolding matching_def by simp
 
+lemma partitioned_bipartite_empty[simp]: "partitioned_bipartite {} X"
+  unfolding partitioned_bipartite_def by simp
+
+lemma partitioned_bipartiteI[intro]:
+  assumes "graph_abs E"
+  assumes "\<And>e. e \<in> E \<Longrightarrow> \<exists>u v. e = {u,v} \<and> u \<in> X \<and> v \<in> Vs E - X"
+  shows "partitioned_bipartite E X"
+  using assms
+  unfolding partitioned_bipartite_def
+  by (auto simp: graph_abs_def)
+
+lemma partitioned_bipartite_graph_absD:
+  assumes "partitioned_bipartite E X"
+  shows "graph_abs E"
+  using assms
+  unfolding partitioned_bipartite_def
+  by (auto intro: graph_abs.intro)
+
+lemma partitioned_bipartiteE[elim?]:
+  assumes "partitioned_bipartite E X"
+  assumes "e \<in> E"
+  obtains u v where "e = {u,v}" "u \<in> X" "v \<in> Vs E - X"
+  using assms
+  unfolding partitioned_bipartite_def
+  by fast
+
 type_synonym 'a graph = "'a set set"
 
 text \<open>For now we don't care about distinctness of the "ranking" list, as we only need the order
   induced by the list.\<close>
 abbreviation "rank \<sigma> v \<equiv> index \<sigma> v"
 
-abbreviation "arriving_U us \<equiv> set (map fst us)"
-abbreviation "arriving_V us \<equiv> \<Union>(set (map snd us))"
+abbreviation "arriving_U us \<equiv> fst ` set us"
+abbreviation "arriving_V us \<equiv> \<Union> (snd ` set us)"
 
 definition wf_input :: "'a list \<Rightarrow> ('a \<times> 'a set) list \<Rightarrow> bool" where
   "wf_input \<sigma> us \<equiv> 
@@ -39,6 +70,10 @@ definition wf_input :: "'a list \<Rightarrow> ('a \<times> 'a set) list \<Righta
     distinct \<sigma> \<and> 
     distinct (map fst us)"
 
+fun neighbors_of :: "'a \<Rightarrow> ('a \<times> 'a set) list \<Rightarrow> 'a set" where
+  "neighbors_of _ [] = {}"
+| "neighbors_of u ((v,ns)#vs) = (if u = v then ns else neighbors_of u vs)"
+
 fun step :: "'a list \<Rightarrow> 'a graph \<Rightarrow> 'a \<Rightarrow> 'a set \<Rightarrow> 'a graph" where
   "step [] M _ _ = M"
 | "step (v#vs) M u neighbors = (
@@ -46,6 +81,13 @@ fun step :: "'a list \<Rightarrow> 'a graph \<Rightarrow> 'a \<Rightarrow> 'a se
     then insert {u,v} M
     else step vs M u neighbors
   )"
+
+lemma step_ConsI:
+  assumes "v \<in> ns \<Longrightarrow> v \<notin> Vs M \<Longrightarrow> P (insert {u,v} M)"
+  assumes "v \<notin> ns \<or> v \<in> Vs M \<Longrightarrow> P (step vs M u ns)"
+  shows "P (step (v#vs) M u ns)"
+  using assms
+  by auto
 
 \<comment> \<open>"Unfold" fold definition to generalize over accumulator.\<close>
 fun ranking_aux :: "'a list \<Rightarrow> ('a \<times> 'a set) list \<Rightarrow> 'a graph \<Rightarrow> 'a graph" where
@@ -57,6 +99,35 @@ definition ranking :: "'a list \<Rightarrow> ('a \<times> 'a set) list \<Rightar
 
 lemma ranking_PI: "P (ranking_aux \<sigma> us {}) \<Longrightarrow> P (ranking \<sigma> us)"
   unfolding ranking_def .
+
+text \<open>The following invariant is maintained by the (steps of the) ranking algorithm.\<close>
+\<comment> \<open>TODO: reconsider the wellformedness of the input in the invariant. It was put there, since the
+  the invariant is only preserved under (some conditions of) wellformedness.\<close>
+definition ranking_inv :: "'a list \<Rightarrow> ('a \<times> 'a set) list \<Rightarrow> 'a graph \<Rightarrow> bool" where
+  "ranking_inv \<sigma> us M \<equiv> wf_input \<sigma> us \<and> matching M \<and> partitioned_bipartite M (set \<sigma>) \<and> 
+    Vs M - set \<sigma> \<subseteq> arriving_U us"
+
+lemma ranking_invI[intro?]:
+  assumes "wf_input \<sigma> us"
+  assumes "matching M"
+  assumes "partitioned_bipartite M (set \<sigma>)"
+  assumes "Vs M - set \<sigma> \<subseteq> arriving_U us"
+  shows "ranking_inv \<sigma> us M"
+  using assms
+  unfolding ranking_inv_def
+  by auto
+
+lemma ranking_invD:
+  assumes "ranking_inv \<sigma> us M"
+  shows "wf_input \<sigma> us" "matching M" "partitioned_bipartite M (set \<sigma>)" "Vs M - set \<sigma> \<subseteq> arriving_U us"
+  using assms
+  unfolding ranking_inv_def
+  by auto
+
+lemma ranking_inv_subset_\<sigma>: "ranking_inv \<sigma> us M \<Longrightarrow> Vs M - arriving_U us \<subseteq> set \<sigma>"
+  unfolding ranking_inv_def
+  by blast
+
 
 fun offline_graph :: "('a \<times> 'a set) list \<Rightarrow> 'a graph" where
   "offline_graph [] = {}"
@@ -77,11 +148,12 @@ lemma wf_input_arriving_disjoint: "wf_input \<sigma> us \<Longrightarrow> arrivi
 lemma wf_input_tl: "wf_input \<sigma> (u # us) \<Longrightarrow> wf_input \<sigma> us"
   unfolding wf_input_def by auto
 
-lemma wf_input_hd: "wf_input \<sigma> ((u,ns) # us) \<Longrightarrow> u \<notin> ns \<and> finite ns \<and> u \<notin> set \<sigma>"
+lemma wf_input_hd: "wf_input \<sigma> ((u,ns) # us) \<Longrightarrow> u \<notin> ns \<and> finite ns \<and> u \<notin> set \<sigma> \<and> ns \<subseteq> set \<sigma>"
   unfolding wf_input_def by (auto intro: finite_subset)
 
 lemma wf_input_hd': "wf_input \<sigma> (u#us) \<Longrightarrow> fst u \<notin> snd u \<and> finite (snd u) \<and> fst u \<notin> set \<sigma>"
   unfolding wf_input_def by (auto intro: finite_subset)
+
 
 lemma edge_in_step:
   assumes "e \<in> step \<sigma> M u ns"
@@ -99,8 +171,24 @@ lemma edge_in_ranking_aux:
    apply (drule edge_in_step, blast)
   by (metis step_mono vs_member)
 
-lemma vs_step: "Vs (step \<sigma> M u ns) \<subseteq> {u} \<union> set \<sigma> \<union> Vs M"
-  by (induction \<sigma> M u ns rule: step.induct) (auto simp: Vs_def)
+lemma vs_step: "v \<in> Vs (step \<sigma> M u ns) \<Longrightarrow> v = u \<or> v \<in> set \<sigma> \<or> v \<in> Vs M"
+  by (induction \<sigma> M u ns rule: step.induct) (auto split: if_splits simp: Vs_def)
+
+lemma vs_step': "v \<in> Vs (step \<sigma> M u ns) \<Longrightarrow> v \<in> Vs M \<or> v \<in> Vs {{u,v}| v. v \<in> ns}"
+  by (induction \<sigma> M u ns rule: step.induct) (auto split: if_splits simp: Vs_def)
+
+lemma vs_ranking_aux: "v \<in> Vs (ranking_aux \<sigma> us M) \<Longrightarrow> v \<in> Vs M \<or> v \<in> Vs (offline_graph us)"
+proof (induction \<sigma> us M rule: ranking_aux.induct)
+  case (2 \<sigma> u ns us M)
+  then show ?case 
+    by (auto dest: vs_step')
+qed simp
+
+lemma vs_offline_graph: "v \<in> Vs (offline_graph us) \<Longrightarrow> v \<in> arriving_U us \<or> v \<in> arriving_V us"
+  by (induction us rule: offline_graph.induct) (auto simp: Vs_def)
+
+lemma vs_compr: "Vs {{u, v} |v. v \<in> ns} = (if ns = {} then {} else {u} \<union> ns)"
+  unfolding Vs_def by auto
 
 lemma graph_abs_step:
   assumes "graph_abs M"
@@ -110,13 +198,42 @@ lemma graph_abs_step:
   by (induction \<sigma>) auto
 
 lemma matching_step:
-  assumes "graph_abs M"
   assumes "matching M"
   assumes "u \<notin> set \<sigma>"
   assumes "u \<notin> Vs M"
   shows "matching (step \<sigma> M u ns)"
   using assms
   by (induction \<sigma>) (auto simp: matching_def)
+
+lemma partitioned_bipartite_step:
+  assumes "partitioned_bipartite M (set \<sigma>)"
+  assumes "u \<notin> set \<sigma>"
+  shows "partitioned_bipartite (step \<sigma> M u ns) (set \<sigma>)"
+  using assms
+proof (induction \<sigma>)
+  case (Cons a \<sigma>)
+  then have graph_abs: "graph_abs (step \<sigma> M u ns)"
+    by (auto dest: partitioned_bipartite_graph_absD intro: graph_abs_step)
+  show ?case
+    apply (rule step_ConsI)
+    apply rule
+      apply (metis Cons.prems(2) assms(1) graph_abs_insert list.set_intros(1) partitioned_bipartite_graph_absD)
+     apply (smt (verit, del_insts) Cons.prems(1) Cons.prems(2) Diff_iff edges_are_Vs insert_commute insert_iff list.set(2) partitioned_bipartiteE)
+    apply rule
+     apply (rule graph_abs)
+    by (smt (verit, del_insts) Cons.prems(1) Cons.prems(2) Diff_iff IntE edge_in_step edges_are_Vs insertCI insert_commute list.set(2) partitioned_bipartiteE)
+qed simp
+
+lemma ranking_inv_step:
+  assumes "wf_input \<sigma> ((u,ns)#us)"
+  assumes "ranking_inv \<sigma> us M"
+  shows "ranking_inv \<sigma> ((u,ns)#us) (step \<sigma> M u ns)"
+  using assms
+  unfolding ranking_inv_def
+  apply (auto intro!: matching_step partitioned_bipartite_step dest: wf_input_hd)
+  apply (metis (no_types, hide_lams) DiffI assms(1) distinct.simps(2) fst_conv list.simps(9) set_map subset_iff wf_input_def wf_input_hd)
+  by (metis (no_types, lifting) DiffI UnE insert_absorb singleton_insert_inj_eq subset_iff vs_step)
+
 
 lemma wf_input_graph_abs_ranking_aux:
   assumes "graph_abs M"
@@ -125,8 +242,6 @@ lemma wf_input_graph_abs_ranking_aux:
   using assms
   by (induction us arbitrary: M) (auto simp: wf_input_def graph_abs_step)
 
-lemma Int_empty_rev_mono: "A \<inter> C = {} \<Longrightarrow> B \<subseteq> C \<Longrightarrow> A \<inter> B = {}"
-  by blast
 
 lemma wf_input_matching_ranking_aux:
   assumes "graph_abs M"
@@ -142,15 +257,38 @@ proof (induction \<sigma> us M rule: ranking_aux.induct)
   have disjoint': "arriving_U us \<inter> ({u} \<union> set \<sigma> \<union> Vs M) = {}"
     using "2.prems"
     unfolding wf_input_def
-    by (simp add:  Int_Un_distrib Int_commute)
+    by (simp add: Int_Un_distrib Int_commute)
 
   then have "arriving_U us \<inter> Vs (step \<sigma> M u ns) = {}"
-    by (rule Int_empty_rev_mono[OF _ vs_step])
+    by (smt (z3) Int_Un_distrib disjoint_iff insertCI sup_bot.neutr_eq_iff vs_step)
 
   then show ?case
     using "2.IH" 1
     by simp
 qed auto
+
+lemma wf_input_partitioned_bipartite_ranking_aux:
+  assumes "wf_input \<sigma> us"
+  assumes "partitioned_bipartite M (set \<sigma>)"
+  shows "partitioned_bipartite (ranking_aux \<sigma> us M) (set \<sigma>)"
+  using assms
+  by (induction \<sigma> us M rule: ranking_aux.induct)
+     (auto dest: partitioned_bipartite_step wf_input_hd wf_input_tl)
+
+
+lemma wf_input_ranking_inv_ranking_aux:
+  assumes "wf_input \<sigma> us"
+  assumes "ranking_inv \<sigma> [] M"
+  shows "ranking_inv \<sigma> us (ranking_aux \<sigma> us M)"
+  using assms
+  apply (auto intro!: ranking_invI wf_input_matching_ranking_aux wf_input_partitioned_bipartite_ranking_aux 
+        dest: ranking_invD partitioned_bipartite_graph_absD wf_input_tl)
+  apply (metis empty_iff empty_set image_empty partitioned_bipartiteE ranking_inv_def subsetD vs_member)
+  apply (drule vs_ranking_aux)
+  apply auto
+  using ranking_inv_subset_\<sigma> apply fastforce
+  by (meson in_mono vs_offline_graph wf_input_def)
+
 
 lemma wf_input_graph_abs_ranking:
   assumes "wf_input \<sigma> us"
@@ -170,6 +308,43 @@ lemma wf_input_graph_abs_offline_graph:
   using assms
   by (induction us rule: offline_graph.induct) (auto dest: wf_input_tl wf_input_hd)
 
+lemma wf_input_partitioned_bipartite_offline_graph:
+  assumes "wf_input \<sigma> us"
+  shows "partitioned_bipartite (offline_graph us) (set \<sigma>)"
+  using assms
+proof (induction us rule: offline_graph.induct)
+  case (2 u ns us)
+  show ?case 
+  proof (intro partitioned_bipartiteI)
+    show "graph_abs (offline_graph ((u, ns) # us))"
+      using 2 wf_input_graph_abs_offline_graph by blast
+    show "\<And>e. e \<in> offline_graph ((u, ns) # us) \<Longrightarrow> \<exists>u' v. e = {u', v} \<and> u' \<in> set \<sigma> \<and> v \<in> Vs (offline_graph ((u, ns) # us)) - set \<sigma>"
+    proof -
+      fix e
+      assume "e \<in> offline_graph ((u, ns) # us)"
+      then have "e \<in> offline_graph us \<or> e \<in> {{u, v}| v. v \<in> ns}" by auto
+      then consider (ind) "e \<in> offline_graph us" | (new) "e \<in> {{u, v}| v. v \<in> ns}" by blast
+      then show "\<exists>u' v. e = {u', v} \<and> u' \<in> set \<sigma> \<and> v \<in> Vs (offline_graph ((u, ns) # us)) - set \<sigma>" 
+      proof cases
+        case ind
+        then show ?thesis
+          by (smt (verit) "2.IH" "2.prems" DiffD2 DiffI \<open>e \<in> offline_graph ((u, ns) # us)\<close> edges_are_Vs insert_commute partitioned_bipartiteE wf_input_tl)
+      next
+        case new
+        then obtain v where "v \<in> ns" "e = {u,v}" by blast
+        then have "v \<in> set \<sigma>" "u \<notin> set \<sigma>"
+          using 2
+          by (auto dest: wf_input_hd)
+        have "u \<in> Vs (offline_graph ((u, ns) # us))"
+          by (metis \<open>e = {u, v}\<close> \<open>e \<in> offline_graph ((u, ns) # us)\<close> edges_are_Vs)
+        then show ?thesis
+          using \<open>e = {u, v}\<close> \<open>u \<notin> set \<sigma>\<close> \<open>v \<in> set \<sigma>\<close> by blast
+      qed
+    qed
+  qed
+qed auto
+
+  
 
 lemma in_step_elim:
   assumes "e \<in> step \<sigma> M u ns"
@@ -177,9 +352,6 @@ lemma in_step_elim:
   obtains v where "e = {u,v}" "v \<in> ns" "v \<in> set \<sigma>" "v \<notin> Vs M"
   using assms edge_in_step
   by force
-
-lemma step_lowest_rank: "set \<sigma> \<inter> ns \<noteq> {} \<Longrightarrow> step \<sigma> {} u ns = {{u, \<sigma> ! Min (rank \<sigma> ` ns)}}"
-  sorry
 
 
 lemma ranking_aux_subset_offline_graph:
@@ -192,5 +364,172 @@ lemma "x \<in> ranking \<sigma> us \<Longrightarrow> x \<in> offline_graph us"
   unfolding ranking_def
   by (auto dest: ranking_aux_subset_offline_graph)
 
+
+lemma step_lowest_rank:
+  assumes "u \<notin> set \<sigma>"
+  assumes "u \<notin> Vs M"
+  assumes "w \<in> set \<sigma>" "w \<in> ns" "w \<notin> Vs M"
+  assumes "{u,v} \<in> step \<sigma> M u ns"
+  shows "rank \<sigma> v \<le> rank \<sigma> w"
+  using assms
+  apply (induction \<sigma>)
+   apply simp_all
+  by (metis doubleton_eq_iff insert_iff vs_member)
+
+lemma neighbors_of_Cons:
+  assumes "u \<noteq> u'"
+  assumes "w \<in> neighbors_of u ((u', ns) # us)"
+  shows "w \<in> neighbors_of u us"
+  using assms
+  by (induction us) auto
+
+lemma ranking_aux_hd_ineq:
+  assumes "wf_input \<sigma> ((u', ns) # us)"
+  assumes "v \<in> set \<sigma>"
+  assumes "u \<notin> Vs (step \<sigma> M u' ns)"
+  assumes "{u, v} \<in> ranking_aux \<sigma> ((u', ns) # us) M"
+  shows "u \<noteq> u'"
+proof (rule ccontr, simp)
+  assume "u = u'"
+  have "u \<notin> Vs M" using assms
+    by (meson step_mono vs_transport)
+  have "u \<notin> arriving_U us"
+    by (metis (no_types, hide_lams) \<open>u = u'\<close> assms(1) distinct.simps(2) fst_conv list.simps(9) set_map wf_input_def)
+  show False
+    by (metis (no_types, lifting) \<open>u = u'\<close> \<open>u \<notin> arriving_U us\<close> assms(1) assms(3) assms(4) edges_are_Vs ranking_aux.simps(2) subset_eq vs_offline_graph vs_ranking_aux wf_input_def wf_input_hd wf_input_tl)
+qed
+
+
+lemma u_in_ranking_aux:
+  assumes "wf_input \<sigma> us"
+  assumes "partitioned_bipartite M (set \<sigma>)"
+  assumes "v \<in> set \<sigma>"
+  assumes "u \<notin> Vs M"
+  assumes "{u,v} \<in> ranking_aux \<sigma> us M"
+  shows "u \<notin> set \<sigma>"
+  by (metis DiffD2 assms(1) assms(2) assms(3) assms(5) doubleton_eq_iff partitioned_bipartiteE wf_input_partitioned_bipartite_ranking_aux)
+
+lemma u_in_stepE:
+  assumes "u \<in> Vs (step \<sigma> M u ns)"
+  assumes "u \<notin> Vs M"
+  assumes "u \<notin> set \<sigma>"
+  obtains v where "u \<noteq> v" "{u,v} \<in> step \<sigma> M u ns" "v \<in> ns" "v \<in> set \<sigma>"
+  using assms
+  by (induction \<sigma> M u ns rule: step.induct) (auto split: if_splits)
+
+lemma vertex_in_step_edge_in_step:
+  assumes "wf_input \<sigma> ((u,ns)#us)"
+  assumes "partitioned_bipartite M (set \<sigma>)"
+  assumes "matching M"
+  assumes "arriving_U ((u,ns)#us) \<inter> Vs M = {}"
+  assumes "u \<notin> Vs M"
+  assumes "v \<in> set \<sigma>"
+  assumes "u \<in> Vs (step \<sigma> M u ns)"
+  assumes "{u,v} \<in> ranking_aux \<sigma> ((u,ns)#us) M"
+  shows "{u,v} \<in> step \<sigma> M u ns"
+proof -
+  have "u \<notin> set \<sigma>"
+    by (meson assms(1) wf_input_hd)
+  with assms obtain v' where "u \<noteq> v'" "{u,v'} \<in> step \<sigma> M u ns" "v' \<in> ns" "v' \<in> set \<sigma>"
+    by (auto elim: u_in_stepE)
+  have "v' = v" 
+  proof (rule ccontr)
+    assume "v' \<noteq> v"
+    then have "{u,v'} \<in> ranking_aux \<sigma> ((u,ns)#us) M"
+      by (simp add: \<open>{u, v'} \<in> step \<sigma> M u ns\<close> ranking_aux_mono)
+    have "matching (ranking_aux \<sigma> ((u,ns)#us) M)"
+      by (meson assms(1) assms(2) assms(3) assms(4) partitioned_bipartite_graph_absD wf_input_matching_ranking_aux)
+    then show False 
+      by (metis \<open>v' \<noteq> v\<close> \<open>{u, v'} \<in> ranking_aux \<sigma> ((u, ns) # us) M\<close> assms(8) doubleton_eq_iff insertI1 matching_unique_match)
+  qed
+  then show ?thesis
+    using \<open>{u, v'} \<in> step \<sigma> M u ns\<close> by auto
+qed
+
+
+lemma wf_input_arriving_U_disjoint_Cons:
+  assumes "wf_input \<sigma> ((u,ns)#us)"
+  assumes "arriving_U ((u,ns)#us) \<inter> Vs M = {}"
+  shows "arriving_U us \<inter> Vs (step \<sigma> M u ns) = {}"
+proof (rule ccontr)
+  assume "arriving_U us \<inter> Vs (step \<sigma> M u ns) \<noteq> {}"
+  then obtain u' where "u' \<in> arriving_U us" "u' \<in> Vs (step \<sigma> M u ns)"
+    by blast
+  then consider "u' = u" | "u' \<in> Vs M"
+    by (metis assms(1) disjoint_iff vs_step wf_input_def wf_input_tl)
+  then show False
+  proof cases
+    case 1
+    then show ?thesis
+      by (metis (no_types, hide_lams) \<open>u' \<in> arriving_U us\<close> assms(1) distinct.simps(2) fst_conv list.map(2) set_map wf_input_def)
+  next
+    case 2
+    then show ?thesis
+      using \<open>u' \<in> arriving_U us\<close> assms(2) by fastforce
+  qed
+qed
+
+lemma ranking_aux_lowest_rank:
+  assumes "wf_input \<sigma> us"
+  assumes "u \<notin> Vs M"
+  assumes "v \<in> set \<sigma>" \<comment> \<open>hence, u is the node that arrives\<close>
+  assumes "w \<in> set \<sigma>" "w \<in> neighbors_of u us" "w \<notin> Vs M" "w \<notin> Vs (ranking_aux \<sigma> us M)"
+  assumes "{u,v} \<in> ranking_aux \<sigma> us M"
+  assumes "partitioned_bipartite M (set \<sigma>)"
+  assumes "matching M"
+  assumes "arriving_U us \<inter> Vs M = {}"
+  shows "rank \<sigma> v \<le> rank \<sigma> w"
+  using assms
+proof (induction \<sigma> us M rule: ranking_aux.induct)
+  case (2 \<sigma> u' ns us M)
+
+  have "u \<notin> set \<sigma>"
+    by (meson "2.prems"(1) "2.prems"(2) "2.prems"(3) "2.prems"(8) "2.prems"(9) u_in_ranking_aux)
+
+  consider (ind) "u \<notin> Vs (step \<sigma> M u' ns)" | (new) "u \<in> Vs (step \<sigma> M u' ns)" by blast
+  then show ?case
+  proof cases
+    case ind
+    have "w \<in> set \<sigma>" 
+      using "2.prems"(4) by blast
+    have "w \<in> neighbors_of u us"
+      apply (rule neighbors_of_Cons[where u' = u'])
+       apply (metis "2.prems"(1) "2.prems"(3) "2.prems"(8) ind ranking_aux_hd_ineq wf_input_hd)
+      using "2.prems"(5) by blast
+    have "w \<notin> Vs (step \<sigma> M u' ns)"
+      by (metis "2.prems"(7) ranking_aux.simps(2) ranking_aux_mono vs_member_elim vs_member_intro)
+    have "arriving_U us \<inter> Vs (step \<sigma> M u' ns) = {}"
+      by (meson "2.prems"(1) "2.prems"(11) wf_input_arriving_U_disjoint_Cons)
+    show ?thesis
+      apply (rule "2.IH")
+      using "2.prems"(1) wf_input_tl apply blast
+      apply (simp_all add: "2.prems" ind \<open>w \<in> neighbors_of u us\<close> \<open>w \<notin> Vs (step \<sigma> M u' ns)\<close> \<open>arriving_U us \<inter> Vs (step \<sigma> M u' ns) = {}\<close>)
+      using "2.prems"(7) apply force
+      using "2.prems"(8) apply force
+        apply (meson "2.prems"(1) "2.prems"(9) partitioned_bipartite_step wf_input_hd)
+       apply (metis "2.prems"(1) "2.prems"(10) "2.prems"(11) disjoint_iff fst_conv image_eqI list.set_intros(1) matching_step wf_input_hd)
+      done
+  next
+    case new
+    have "u' = u"
+      by (metis "2.prems"(2) \<open>u \<notin> set \<sigma>\<close> new vs_step)
+    then have "{u,v} \<in> step \<sigma> M u ns"
+      by (metis "2.prems"(1) "2.prems"(10) "2.prems"(11) "2.prems"(2) "2.prems"(3) "2.prems"(8) "2.prems"(9) new vertex_in_step_edge_in_step)
+    have "w \<in> ns"
+      using "2.prems"(5) \<open>u' = u\<close> by auto
+    show ?thesis
+      by (meson "2.prems"(2) "2.prems"(4) "2.prems"(6) \<open>u \<notin> set \<sigma>\<close> \<open>w \<in> ns\<close> \<open>{u, v} \<in> step \<sigma> M u ns\<close> step_lowest_rank)
+  qed
+qed simp
+
+
+lemma ranking_lowest_rank:
+  assumes "wf_input \<sigma> us"
+  assumes "v \<in> set \<sigma>"
+  assumes "w \<in> set \<sigma>" "w \<in> neighbors_of u us" "w \<notin> Vs (ranking \<sigma> us)"
+  assumes "{u,v} \<in> ranking \<sigma> us"
+  shows "rank \<sigma> v \<le> rank \<sigma> w"
+  using assms
+  by (intro ranking_aux_lowest_rank[where u = u and M = "{}"]) (simp_all add: ranking_def)
 
 end
